src/SynthesisFacts.v
@@ -103,76 +103,6 @@ Proof.
   reflexivity.
 Qed.
 
-Theorem simulation_pmsgs_compositional:
-  forall {StateS LabelS: Type} `{HasInit StateS} `{HasLabel LabelS}
-         (stepS: Step StateS LabelS)
-         impl1 impl2 spec simR simP
-         (Hidx: indicesOf impl1 = indicesOf impl2)
-         (Hsim1: Simulates step_seq stepS simR simP impl1 spec)
-         (Hsim2: Simulates step_seq stepS simR simP impl2 spec)
-         impl (Hii: indicesOf impl = indicesOf impl1)
-         (Himplp:
-            forall pmsg iobj,
-              In pmsg (obj_trs iobj) ->
-              In iobj (sys_objs impl) ->
-              exists obj,
-                obj_idx obj = obj_idx iobj /\
-                In pmsg (obj_trs obj) /\
-                In obj (sys_objs impl1 ++ sys_objs impl2)),
-    Simulates step_seq stepS simR simP impl spec.
-Proof.
-  unfold Simulates; intros.
-  specialize (Hsim1 ist1 sst1 H1 ilbl ist2).
-  specialize (Hsim2 ist1 sst1 H1 ilbl ist2).
-
-  destruct ilbl as [|[hdl|]];
-    [apply Hsim1; eapply step_seq_in_pmsgs_weakening; eauto|
-     |inv H2; apply Hsim1; constructor].
-  
-  match goal with
-  | [ |- ?g ] =>
-    assert (Hsp: step_seq impl1 ist1 (IlblOuts (Some hdl) mouts) ist2 \/
-                 step_seq impl2 ist1 (IlblOuts (Some hdl) mouts) ist2 -> g)
-      by (intro Hsp; destruct Hsp; [apply Hsim1; assumption|apply Hsim2; assumption])
-  end.
-  apply Hsp; clear Hsp Hsim1 Hsim2.
-  inv H2.
-
-  - specialize (Himplp _ _ H13 H5); destruct Himplp as [iobj [? [? ?]]].
-    apply in_app_or in H4; destruct H4.
-    + left.
-      replace (extOuts impl) with (extOuts impl1)
-        by (unfold extOuts, isExternal; rewrite Hii; reflexivity).
-      replace (intOuts impl) with (intOuts impl1)
-        by (unfold intOuts, isInternal; rewrite Hii; reflexivity).
-      eapply SsIntInit; eauto.
-      unfold isExternal in *; rewrite <-Hii; assumption.
-    + right.
-      replace (extOuts impl) with (extOuts impl2)
-        by (unfold extOuts, isExternal; rewrite Hii, Hidx; reflexivity).
-      replace (intOuts impl) with (intOuts impl2)
-        by (unfold intOuts, isInternal; rewrite Hii, Hidx; reflexivity).
-      eapply SsIntInit; eauto.
-      unfold isExternal in *; rewrite <-Hidx, <-Hii; assumption.
-
-  - specialize (Himplp _ _ H13 H5); destruct Himplp as [iobj [? [? ?]]].
-    apply in_app_or in H4; destruct H4.
-    + left.
-      replace (extOuts impl) with (extOuts impl1)
-        by (unfold extOuts, isExternal; rewrite Hii; reflexivity).
-      replace (intOuts impl) with (intOuts impl1)
-        by (unfold intOuts, isInternal; rewrite Hii; reflexivity).
-      eapply SsIntFwd; eauto.
-      unfold isInternal; rewrite <-Hii; assumption.
-    + right.
-      replace (extOuts impl) with (extOuts impl2)
-        by (unfold extOuts, isExternal; rewrite Hii, Hidx; reflexivity).
-      replace (intOuts impl) with (intOuts impl2)
-        by (unfold intOuts, isInternal; rewrite Hii, Hidx; reflexivity).
-      eapply SsIntFwd; eauto.
-      unfold isInternal; rewrite <-Hidx, <-Hii; assumption.
-Qed.
-
 Lemma buildRawSys_indicesOf:
   forall sys, indicesOf sys = indicesOf (buildRawSys sys).
 Proof.
@@ -245,25 +175,6 @@ Lemma addPMsgsSys_pmsg_in:
 Proof.
   intros; destruct sys as [obs chns]; simpl in *.
   apply addPMsgs_pmsg_in; auto.
-Qed.
-
-Corollary simulation_pmsgs_added:
-  forall {StateS LabelS: Type} `{HasInit StateS} `{HasLabel LabelS}
-         (stepS: Step StateS LabelS)
-         impl pmsgs spec simR simP
-         (Hsim1: Simulates step_seq stepS simR simP impl spec)
-         (Hsim2: Simulates step_seq stepS simR simP
-                           (addPMsgsSys pmsgs (buildRawSys impl)) spec),
-    Simulates step_seq stepS simR simP (addPMsgsSys pmsgs impl) spec.
-Proof.
-  intros.
-  eapply simulation_pmsgs_compositional
-    with (impl1:= impl) (impl2:= addPMsgsSys pmsgs (buildRawSys impl)); eauto.
-  - rewrite addPMsgsSys_indices.
-    apply buildRawSys_indicesOf.
-  - apply addPMsgsSys_indices.
-  - clear; intros.
-    apply addPMsgsSys_pmsg_in; auto.
 Qed.
 
 Lemma addPMsgsSys_buildRawSys_sublist:
